Divisor.lean
@@ -54,6 +54,7 @@ import Divisor.FrobDescentHelpers
 import Divisor.SlopeChoice
 import Divisor.GeometricSoundness
 import Divisor.IsHonestForBinary
+import Divisor.SafeSupport
 import Divisor.Hasse
 import Divisor.Sketch.ChordFiberProductConcrete
 import Divisor.Sketch.ChordFiberGeometry
